src/tls/MITLS.Repr.CertificateVerify12.fst
@@ -27,7 +27,7 @@ module MITLS.Repr.CertificateVerify12
 module LP = LowParse.Low.Base
 module B = LowStar.Monotonic.Buffer
 module HS = FStar.HyperStack
-module R = MITLS.Repr
+module R = LowParse.Repr
 open FStar.Integers
 open FStar.HyperStack.ST
 
@@ -35,5 +35,5 @@ module CV12 = Parsers.CertificateVerify12
 
 let t = CV12.certificateVerify12
 
-let repr (b:LowParse.Ptr.const_slice) =
-  R.repr_p t b CV12.certificateVerify12_parser
+let ptr = R.repr_ptr_p t CV12.certificateVerify12_parser
+let pos (b:R.const_slice) = R.repr_pos_p t b CV12.certificateVerify12_parser
