src/tls/MITLS.Repr.Handshake12.fst
@@ -34,7 +34,7 @@ module LP = LowParse.Low.Base
 module LS = LowParse.SLow.Base
 module B  = LowStar.Buffer
 module HS = FStar.HyperStack
-module R  = MITLS.Repr
+module R  = LowParse.Repr
 
 open FStar.Integers
 open FStar.HyperStack.ST
@@ -53,54 +53,64 @@ module FinRepr = MITLS.Repr.Finished12
 
 type t = HSM12.handshake12
 
-type repr (b:R.const_slice) =
-  R.repr_p t b HSM12.handshake12_parser32
+type ptr =
+  R.repr_ptr_p t HSM12.handshake12_parser
 
-let is_hr (#b:R.const_slice) (r:repr b) : GTot bool =
-  HSM12.M12_hello_request? (R.value r)
+type pos (b:R.const_slice) =
+  R.repr_pos_p t b HSM12.handshake12_parser
 
-let is_c (#b:R.const_slice) (r:repr b) : GTot bool =
-  HSM12.M12_certificate? (R.value r)
+let is_hr (#b:R.const_slice) (r:pos b) : GTot bool =
+  HSM12.M12_hello_request? (R.value_pos r)
 
-let is_ske (#b:R.const_slice) (r:repr b) : GTot bool =
-  HSM12.M12_server_key_exchange? (R.value r)
+let is_c (#b:R.const_slice) (r:pos b) : GTot bool =
+  HSM12.M12_certificate? (R.value_pos r)
 
-let is_cr (#b:R.const_slice) (r:repr b) : GTot bool =
-  HSM12.M12_certificate_request? (R.value r)
+let is_ske (#b:R.const_slice) (r:pos b) : GTot bool =
+  HSM12.M12_server_key_exchange? (R.value_pos r)
 
-let is_shd (#b:R.const_slice) (r:repr b) : GTot bool =
-  HSM12.M12_server_hello_done? (R.value r)
+let is_cr (#b:R.const_slice) (r:pos b) : GTot bool =
+  HSM12.M12_certificate_request? (R.value_pos r)
 
-let is_cv (#b:R.const_slice) (r:repr b) : GTot bool =
-  HSM12.M12_certificate_verify? (R.value r)
+let is_shd (#b:R.const_slice) (r:pos b) : GTot bool =
+  HSM12.M12_server_hello_done? (R.value_pos r)
 
-let is_cke (#b:R.const_slice) (r:repr b) : GTot bool =
-  HSM12.M12_client_key_exchange? (R.value r)
+let is_cv (#b:R.const_slice) (r:pos b) : GTot bool =
+  HSM12.M12_certificate_verify? (R.value_pos r)
 
-let is_nst (#b:R.const_slice) (r:repr b) : GTot bool =
-  HSM12.M12_new_session_ticket? (R.value r)
+let is_cke (#b:R.const_slice) (r:pos b) : GTot bool =
+  HSM12.M12_client_key_exchange? (R.value_pos r)
 
-let is_fin (#b:R.const_slice) (r:repr b) : GTot bool =
-  HSM12.M12_finished? (R.value r)
+let is_nst (#b:R.const_slice) (r:pos b) : GTot bool =
+  HSM12.M12_new_session_ticket? (R.value_pos r)
 
-type hr12_repr (b:R.const_slice) = m:repr b{is_hr m}
-type c12_repr (b:R.const_slice) = m:repr b{is_c m}
-type ske12_repr (b:R.const_slice) = m:repr b{is_ske m}
-type cr12_repr (b:R.const_slice) = m:repr b{is_cr m}
-type shd12_repr (b:R.const_slice) = m:repr b{is_shd m}
-type cv12_repr (b:R.const_slice) = m:repr b{is_cv m}
-type cke12_repr (b:R.const_slice) = m:repr b{is_cke m}
-type nst12_repr (b:R.const_slice) = m:repr b{is_nst m}
-type fin12_repr (b:R.const_slice) = m:repr b{is_fin m}
+let is_fin (#b:R.const_slice) (r:pos b) : GTot bool =
+  HSM12.M12_finished? (R.value_pos r)
+
+type hr12_pos (b:R.const_slice) = m:pos b{is_hr m}
+type c12_pos (b:R.const_slice) = m:pos b{is_c m}
+type ske12_pos (b:R.const_slice) = m:pos b{is_ske m}
+type cr12_pos (b:R.const_slice) = m:pos b{is_cr m}
+type shd12_pos (b:R.const_slice) = m:pos b{is_shd m}
+type cv12_pos (b:R.const_slice) = m:pos b{is_cv m}
+type cke12_pos (b:R.const_slice) = m:pos b{is_cke m}
+type nst12_pos (b:R.const_slice) = m:pos b{is_nst m}
+type fin12_pos (b:R.const_slice) = m:pos b{is_fin m}
 
 
 (*
  * Common precondition for functions that return the
  *   reprs for specific instance types
  *)
-unfold let repr_pre (#b:R.const_slice) (r:repr b)
+unfold let repr_pre (#b:R.const_slice) (r:pos b)
   : HS.mem -> Type0
-  = fun h -> R.valid r h
+  = fun h -> R.repr_pos_valid r h
+
+let repr = pos
+
+let end_pos #t #b (r:R.repr_pos t b)
+  : GTot uint_32
+  = let open R in
+    r.start_pos + (Pos?.meta r).len
 
 (*
  * Common postcondition for functions that return the
@@ -108,138 +118,140 @@ unfold let repr_pre (#b:R.const_slice) (r:repr b)
  *)
 unfold let repr_post_common
   (#b:R.const_slice)
-  (#a:Type) (#k:LP.parser_kind) (#p:LP.parser k a) (#p32:LS.parser32 p)
+  (#a:Type) (#k:LP.parser_kind) (#p:LP.parser k a)
   (r:repr b)  //input repr
-  : HS.mem -> R.repr_p a b p32 -> HS.mem -> Type0
+  : HS.mem -> R.repr_pos_p a b p -> HS.mem -> Type0
   = fun h0 rr h1 ->
     let open R in
     B.(modifies loc_none h0 h1) /\
-    valid rr h1 /\  //the returned repr is valid in h1
+    R.repr_pos_valid rr h1 /\  //the returned repr is valid in h1
     r.start_pos <= rr.start_pos /\  //slice indices for the instance repr are contained in the slice indices of r ...
-    rr.end_pos <= r.end_pos  //... useful for framing
+    end_pos rr <= end_pos r  //... useful for framing
 
-let get_hr_repr (#b:R.const_slice) (r:repr b{is_hr r})
-  : Stack (HRRepr.repr b)
+let get_hr_repr (#b:R.const_slice) (r:pos b{is_hr r})
+  : Stack (HRRepr.pos b)
     (requires repr_pre r)
     (ensures  fun h0 rr h1 ->
-      R.value r == HSM12.M12_hello_request (R.value rr) /\
+      R.value_pos r == HSM12.M12_hello_request (R.value_pos rr) /\
       repr_post_common r h0 rr h1)
-  = R.reveal_valid ();
-    let lp_b = R.to_slice b in
-    let pos = HSM12.handshake12_accessor_hello_request lp_b r.R.start_pos in
-    let end_pos = HSM12.handshake12_m12_hello_request_jumper lp_b pos in
+  = admit()// ;
+    // R.reveal_valid ();
+    // let lp_b = R.to_slice b in
+    // let pos = HSM12.handshake12_accessor_hello_request lp_b r.R.start_pos in
+    // let end_pos = HSM12.handshake12_m12_hello_request_jumper lp_b pos in
 
-    R.mk_from_const_slice b pos end_pos HSM12.handshake12_m12_hello_request_parser32
+    // R.mk_repr_pos_from_const_slice b pos end_pos HSM12.handshake12_m12_hello_request_parser32
 
-let get_c_repr (#b:R.const_slice) (r:repr b{is_c r})
-  : Stack (CRepr.repr b)
+let get_c_repr (#b:R.const_slice) (r:pos b{is_c r})
+  : Stack (CRepr.pos b)
     (requires repr_pre r)
     (ensures  fun h0 rr h1 ->
-      let l = Parsers.Certificate12.certificate12_bytesize (R.value rr) in
+      let l = Parsers.Certificate12.certificate12_bytesize (R.value_pos rr) in
       0 <= l /\ l <= 16777215 /\
-      R.value r == HSM12.M12_certificate (R.value rr) /\
+      R.value_pos r == HSM12.M12_certificate (R.value_pos rr) /\
       repr_post_common r h0 rr h1)
-  = R.reveal_valid ();
-    let lp_b = R.to_slice b in
-    let pos = HSM12.handshake12_accessor_certificate lp_b r.R.start_pos in
-    let pos = HSM12.handshake12_m12_certificate_accessor lp_b pos in
-    let end_pos = Parsers.Certificate12.certificate12_jumper lp_b pos in
+  = admit()// ;
+    // R.reveal_valid ();
+    // let lp_b = R.to_slice b in
+    // let pos = HSM12.handshake12_accessor_certificate lp_b r.R.start_pos in
+    // let pos = HSM12.handshake12_m12_certificate_accessor lp_b pos in
+    // let end_pos = Parsers.Certificate12.certificate12_jumper lp_b pos in
 
-    R.mk_from_const_slice b pos end_pos Parsers.Certificate12.certificate12_parser32
+    // R.mk_from_const_slice b pos end_pos Parsers.Certificate12.certificate12_parser32
 
-let get_ske_repr (#b:R.const_slice) (r:repr b{is_ske r})
-  : Stack (SKERepr.repr b)
+let get_ske_repr (#b:R.const_slice) (r:pos b{is_ske r})
+  : Stack (SKERepr.pos b)
     (requires repr_pre r)
     (ensures  fun h0 rr h1 ->
-      R.value r == HSM12.M12_server_key_exchange (R.value rr) /\
+      R.value_pos r == HSM12.M12_server_key_exchange (R.value_pos rr) /\
       repr_post_common r h0 rr h1)
-  = R.reveal_valid ();
-    let lp_b = R.to_slice b in
-    let pos = HSM12.handshake12_accessor_server_key_exchange lp_b r.R.start_pos in
-    let end_pos = HSM12.handshake12_m12_server_key_exchange_jumper lp_b pos in
+  = admit()// R.reveal_valid ();
+    // let lp_b = R.to_slice b in
+    // let pos = HSM12.handshake12_accessor_server_key_exchange lp_b r.R.start_pos in
+    // let end_pos = HSM12.handshake12_m12_server_key_exchange_jumper lp_b pos in
 
-    R.mk_from_const_slice b pos end_pos HSM12.handshake12_m12_server_key_exchange_parser32
+    // R.mk_from_const_slice b pos end_pos HSM12.handshake12_m12_server_key_exchange_parser32
 
-let get_cr_repr (#b:R.const_slice) (r:repr b{is_cr r})
-  : Stack (CRRepr.repr b)
+let get_cr_repr (#b:R.const_slice) (r:pos b{is_cr r})
+  : Stack (CRRepr.pos b)
     (requires repr_pre r)
     (ensures  fun h0 rr h1 ->
-      R.value r == HSM12.M12_certificate_request (R.value rr) /\
+      R.value_pos r == HSM12.M12_certificate_request (R.value_pos rr) /\
       repr_post_common r h0 rr h1)
-  = R.reveal_valid ();
-    let lp_b = R.to_slice b in
-    let pos = HSM12.handshake12_accessor_certificate_request lp_b r.R.start_pos in
-    let pos = HSM12.handshake12_m12_certificate_request_accessor lp_b pos in
-    let end_pos = Parsers.CertificateRequest12.certificateRequest12_jumper lp_b pos in
+  = admit()// R.reveal_valid ();
+    // let lp_b = R.to_slice b in
+    // let pos = HSM12.handshake12_accessor_certificate_request lp_b r.R.start_pos in
+    // let pos = HSM12.handshake12_m12_certificate_request_accessor lp_b pos in
+    // let end_pos = Parsers.CertificateRequest12.certificateRequest12_jumper lp_b pos in
 
-    R.mk_from_const_slice b pos end_pos Parsers.CertificateRequest12.certificateRequest12_parser32
+    // R.mk_from_const_slice b pos end_pos Parsers.CertificateRequest12.certificateRequest12_parser32
 
-let get_shd_repr (#b:R.const_slice) (r:repr b{is_shd r})
-  : Stack (SHDRepr.repr b)
+let get_shd_repr (#b:R.const_slice) (r:pos b{is_shd r})
+  : Stack (SHDRepr.pos b)
     (requires repr_pre r)
     (ensures  fun h0 rr h1 ->
-      R.value r == HSM12.M12_server_hello_done (R.value rr) /\
+      R.value_pos r == HSM12.M12_server_hello_done (R.value_pos rr) /\
       repr_post_common r h0 rr h1)
-  = R.reveal_valid ();
-    let lp_b = R.to_slice b in
-    let pos = HSM12.handshake12_accessor_server_hello_done lp_b r.R.start_pos in
-    let end_pos = HSM12.handshake12_m12_server_hello_done_jumper lp_b pos in
+  = admit()// R.reveal_valid ();
+    // let lp_b = R.to_slice b in
+    // let pos = HSM12.handshake12_accessor_server_hello_done lp_b r.R.start_pos in
+    // let end_pos = HSM12.handshake12_m12_server_hello_done_jumper lp_b pos in
 
-    R.mk_from_const_slice b pos end_pos HSM12.handshake12_m12_server_hello_done_parser32
+    // R.mk_from_const_slice b pos end_pos HSM12.handshake12_m12_server_hello_done_parser32
 
-let get_cv_repr (#b:R.const_slice) (r:repr b{is_cv r})
-  : Stack (CVRepr.repr b)
+let get_cv_repr (#b:R.const_slice) (r:pos b{is_cv r})
+  : Stack (CVRepr.pos b)
     (requires repr_pre r)
     (ensures  fun h0 rr h1 ->
-      R.value r = HSM12.M12_certificate_verify (R.value rr) /\
+      R.value_pos r = HSM12.M12_certificate_verify (R.value_pos rr) /\
       repr_post_common r h0 rr h1)
-  = R.reveal_valid ();
-    let lp_b = R.to_slice b in
-    let pos = HSM12.handshake12_accessor_certificate_verify lp_b r.R.start_pos in
-    let pos = HSM12.handshake12_m12_certificate_verify_accessor lp_b pos in
-    let end_pos = Parsers.CertificateVerify12.certificateVerify12_jumper lp_b pos in
+  = admit()// R.reveal_valid ();
+    // let lp_b = R.to_slice b in
+    // let pos = HSM12.handshake12_accessor_certificate_verify lp_b r.R.start_pos in
+    // let pos = HSM12.handshake12_m12_certificate_verify_accessor lp_b pos in
+    // let end_pos = Parsers.CertificateVerify12.certificateVerify12_jumper lp_b pos in
 
-    R.mk_from_const_slice b pos end_pos Parsers.CertificateVerify12.certificateVerify12_parser32
+    // R.mk_from_const_slice b pos end_pos Parsers.CertificateVerify12.certificateVerify12_parser32
 
-let get_cke_repr (#b:R.const_slice) (r:repr b{is_cke r})
-  : Stack (CKERepr.repr b)
+let get_cke_repr (#b:R.const_slice) (r:pos b{is_cke r})
+  : Stack (CKERepr.pos b)
     (requires repr_pre r)
     (ensures  fun h0 rr h1 ->
-      R.value r == HSM12.M12_client_key_exchange (R.value rr) /\
+      R.value_pos r == HSM12.M12_client_key_exchange (R.value_pos rr) /\
       repr_post_common r h0 rr h1)
-  = R.reveal_valid ();
-    let lp_b = R.to_slice b in
-    let pos = HSM12.handshake12_accessor_client_key_exchange lp_b r.R.start_pos in
-    let end_pos = HSM12.handshake12_m12_client_key_exchange_jumper lp_b pos in
+  = admit()// R.reveal_valid ();
+    // let lp_b = R.to_slice b in
+    // let pos = HSM12.handshake12_accessor_client_key_exchange lp_b r.R.start_pos in
+    // let end_pos = HSM12.handshake12_m12_client_key_exchange_jumper lp_b pos in
 
-    R.mk_from_const_slice b pos end_pos HSM12.handshake12_m12_client_key_exchange_parser32
+    // R.mk_from_const_slice b pos end_pos HSM12.handshake12_m12_client_key_exchange_parser32
 
-let get_nst_repr (#b:R.const_slice) (r:repr b{is_nst r})
-  : Stack (NSTRepr.repr b)
+let get_nst_repr (#b:R.const_slice) (r:pos b{is_nst r})
+  : Stack (NSTRepr.pos b)
     (requires repr_pre r)
     (ensures  fun h0 rr h1 ->
-      R.value r == HSM12.M12_new_session_ticket (R.value rr) /\
+      R.value_pos r == HSM12.M12_new_session_ticket (R.value_pos rr) /\
       repr_post_common r h0 rr h1)
-  = R.reveal_valid ();
-    let lp_b = R.to_slice b in
-    let pos = HSM12.handshake12_accessor_new_session_ticket lp_b r.R.start_pos in
-    let pos = HSM12.handshake12_m12_new_session_ticket_accessor lp_b pos in
-    let end_pos = Parsers.NewSessionTicket12.newSessionTicket12_jumper lp_b pos in
+  = admit()// R.reveal_valid ();
+    // let lp_b = R.to_slice b in
+    // let pos = HSM12.handshake12_accessor_new_session_ticket lp_b r.R.start_pos in
+    // let pos = HSM12.handshake12_m12_new_session_ticket_accessor lp_b pos in
+    // let end_pos = Parsers.NewSessionTicket12.newSessionTicket12_jumper lp_b pos in
 
-    R.mk_from_const_slice b pos end_pos Parsers.NewSessionTicket12.newSessionTicket12_parser32
+    // R.mk_from_const_slice b pos end_pos Parsers.NewSessionTicket12.newSessionTicket12_parser32
 
-let get_fin_repr (#b:R.const_slice) (r:repr b{is_fin r})
-  : Stack (FinRepr.repr b)
+let get_fin_repr (#b:R.const_slice) (r:pos b{is_fin r})
+  : Stack (FinRepr.pos b)
     (requires repr_pre r)
     (ensures  fun h0 rr h1 ->
-      R.value r == HSM12.M12_finished (R.value rr) /\
+      R.value_pos r == HSM12.M12_finished (R.value_pos rr) /\
       repr_post_common r h0 rr h1)
-  = R.reveal_valid ();
-    let lp_b = R.to_slice b in
-    let pos = HSM12.handshake12_accessor_finished lp_b r.R.start_pos in
-    let end_pos = HSM12.handshake12_m12_finished_jumper lp_b pos in
+  = admit()// R.reveal_valid ();
+    // let lp_b = R.to_slice b in
+    // let pos = HSM12.handshake12_accessor_finished lp_b r.R.start_pos in
+    // let end_pos = HSM12.handshake12_m12_finished_jumper lp_b pos in
 
-    R.mk_from_const_slice b pos end_pos HSM12.handshake12_m12_finished_parser32
+    // R.mk_from_const_slice b pos end_pos HSM12.handshake12_m12_finished_parser32
 
 (* Serializer from high-level value via intermediate-level formatter *)
 
@@ -247,7 +259,7 @@ let serialize
   (b:LP.slice R.mut_p R.mut_p{ LP.(b.len <= validator_max_length) })
   (from:R.index (R.of_slice b))
   (x: t)
-: Stack (option (repr (R.of_slice b)))
+  : Stack (option (pos (R.of_slice b)))
     (requires fun h ->
       LP.live_slice h b)
     (ensures fun h0 r h1 ->
@@ -257,9 +269,13 @@ let serialize
         (* not enough space in output slice *)
         Seq.length (LP.serialize HSM12.handshake12_serializer x) > FStar.UInt32.v (b.LP.len - from)
       | Some r ->
-        R.valid r h1 /\
+        R.repr_pos_valid r h1 /\
         r.R.start_pos == from /\
-        R.value r == x
-      end
-    )
-= R.mk_from_serialize b from HSM12.handshake12_parser32 HSM12.handshake12_serializer32 HSM12.handshake12_size32 x
+        R.value_pos r == x
+      end)
+  = R.mk_repr_pos_from_serialize
+        b from
+        HSM12.handshake12_parser32
+        HSM12.handshake12_serializer32
+        HSM12.handshake12_size32
+        x
